feat(C03/S03): solve exercises through 3.3.7
Exercise solutions for §3.3 up to Exercise 3.3.7.

Lean4AnalysisTao/C03_SetTheory/solutions/Solutions_S03_Functions.lean
@@ -168,7 +168,24 @@ end Example_3_3_3
 theorem MyFun.substitute (f : MyFun α β) {x x' : α}
   (hx : x ∈ f.domain) (hx' : x' ∈ f.domain) :
   x = x' → f.eval x hx = f.eval x' hx' := by
-  sorry
+  intro hxx'
+  rcases f.isValidProp x hx with ⟨y, hy, hPxy, hy!⟩
+  rcases f.isValidProp x' hx' with ⟨y', hy', hPx'y', hy'!⟩
+  have hPxy' : f.prop x y' := by
+      rw [hxx']
+      exact hPx'y'
+  have hyy' : y = y' := hy! y' hy' hPxy'
+  have hy' : y' = f.eval x hx := by
+    exact (f.def hx hy').mpr hPxy'
+  have hy : y = f.eval x' hx' := by
+    have hPx'y : f.prop x' y := by
+      rw [← hxx']
+      exact hPxy
+    have := f.def hx' hy
+    exact this.mpr hPx'y
+  rw [← hy]
+  rw [← hy']
+  exact hyy'.symm
 
 -- Example 3.3.5
 example : ∃ (α β : Type) (f : MyFun α β) (x x' : α)
@@ -627,14 +644,14 @@ example : f.isBijective := by
 end Example_3_3_25
 
 -- Remark 3.3.27
-theorem MyFun.exists_unique_of_bijective {α β : Type} (f : MyFun α β)
-  (h : f.isBijective) :
-  ∀ (y : β), y ∈ f.codomain →
+theorem MyFun.exists_unique_of_bijective {α β : Type} {f : MyFun α β}
+  (hf : f.isBijective) :
+  ∀ {y : β}, y ∈ f.codomain →
     ∃ (x : α) (hx : x ∈ f.domain), f.eval x hx = y ∧
-      ∀ (x' : α) (hx' : x' ∈ f.domain), f.eval x' hx' = y → x = x' := by
+      ∀ {x' : α} (hx' : x' ∈ f.domain), f.eval x' hx' = y → x = x' := by
   intro y hy
-  dsimp only [MyFun.isBijective] at h
-  rcases h with ⟨hinj, hsurj⟩
+  dsimp only [MyFun.isBijective] at hf
+  rcases hf with ⟨hinj, hsurj⟩
   dsimp only [MyFun.isSurjective] at hsurj
   rcases hsurj y hy with ⟨x, hx, hxy⟩
   use x, hx, hxy
@@ -644,64 +661,157 @@ theorem MyFun.exists_unique_of_bijective {α β : Type} (f : MyFun α β)
   rw [← hxy'] at hxy
   exact hinj hx hx' hxy
 
-def MyFun.inv {α β : Type} (f : MyFun α β) (h : f.isBijective) :
+def MyFun.inv {α β : Type} (f : MyFun α β) (hf : f.isBijective) :
   MyFun β α := by
   let X : MySet β := f.codomain
   let Y : MySet α := f.domain
   let finv (y : β) (hy : y ∈ X) : α :=
-    (MyFun.exists_unique_of_bijective f h y hy).choose
+    (MyFun.exists_unique_of_bijective hf hy).choose
   let aux : ∀ {y : β} (hy : y ∈ X), finv y hy ∈ Y := by
     intro y hy
     dsimp only [Y]
     dsimp only [finv]
-    rcases (MyFun.exists_unique_of_bijective f h y hy).choose_spec with ⟨hx, h⟩
+    rcases (MyFun.exists_unique_of_bijective hf hy).choose_spec with ⟨hx, h⟩
     exact hx
   exact MyFun.from_fun aux
 
--- theorem MyFun.inv_domain {α β : Type} {f : MyFun α β} (hf : f.isBijective)
---   {fi : MyFun β α} (hfi : fi = MyFun.inv f hf) :
---   fi.codomain = f.domain := by
---   rw [hfi]
---   dsimp only [MyFun.inv]
---   dsimp only [MyFun.from_fun]
 
--- theorem MyFun.inv_codomain {α β : Type} {f : MyFun α β} (hf : f.isBijective)
---   {fi : MyFun β α} (hfi : fi = MyFun.inv f hf) :
---   fi.domain = f.codomain := by
---   rw [hfi]
---   dsimp only [MyFun.inv]
---   dsimp only [MyFun.from_fun]
 
 namespace Exercises
 
 -- Exercise 3.3.1
 example :
   ∀ (f : MyFun α β), f ≃ f := by
-  sorry
+  intro f
+  dsimp only [MyFun.eq]
+  constructor
+  · rfl
+  · constructor
+    · rfl
+    · intro x hxf hxg
+      dsimp only [MyFun.eval]
 
 example :
   ∀ (f g : MyFun α β), (f ≃ g) → (g ≃ f) := by
-  sorry
+  intro f g h
+  dsimp only [MyFun.eq] at h
+  rcases h with ⟨hdom, hcodom, hfg⟩
+  dsimp only [MyFun.eq]
+  constructor
+  · exact hdom.symm
+  · constructor
+    · exact hcodom.symm
+    · intro x hxg hxf
+      exact (hfg hxf hxg).symm
 
 example :
   ∀ (f g h : MyFun α β), (f ≃ g) → (g ≃ h) → (f ≃ h) := by
-  sorry
+  intro f g h hfg hgh
+  dsimp only [MyFun.eq] at hfg
+  rcases hfg with ⟨hdomfg, hcodomfg, hfg⟩
+  dsimp only [MyFun.eq] at hgh
+  rcases hgh with ⟨hdomgh, hcodomgh, hgh⟩
+  dsimp only [MyFun.eq]
+  constructor
+  · rw [hdomfg]
+    exact hdomgh
+  · constructor
+    · rw [hcodomfg]
+      exact hcodomgh
+    · intro x hxf hxh
+      have hxg : x ∈ g.domain := by
+        rw [← hdomfg]
+        exact hxf
+      rw [hfg hxf hxg]
+      exact hgh hxg hxh
 
 example (f f' : MyFun α β) (g g' : MyFun β γ)
   (hfg : f.codomain = g.domain) (hf'g' : f'.codomain = g'.domain) :
   (f ≃ f') → (g ≃ g') → (f.comp g hfg ≃ f'.comp g' hf'g') := by
-  sorry
+  intro hff' hgg'
+  dsimp only [MyFun.eq] at hff'
+  rcases hff' with ⟨hdomff', hcodomff', hff'⟩
+  dsimp only [MyFun.eq] at hgg'
+  rcases hgg' with ⟨hdomgg', hcodomgg', hgg'⟩
+  dsimp only [MyFun.eq]
+  constructor
+  · rw [MyFun.comp.eval.domain]
+    rw [MyFun.comp.eval.domain]
+    exact hdomff'
+  · constructor
+    · rw [MyFun.comp.eval.codomain]
+      rw [MyFun.comp.eval.codomain]
+      exact hcodomgg'
+    · intro x hxf hxf'
+      dsimp only [MyFun.comp]
+      rw [MyFun.from_fun.eval]
+      rw [MyFun.from_fun.eval]
+      dsimp only [MyFun.comp] at hxf
+      dsimp only [MyFun.from_fun] at hxf
+      dsimp only [MyFun.comp] at hxf'
+      dsimp only [MyFun.from_fun] at hxf'
+      have hfxg : f.eval x hxf ∈ g.domain := by
+        rw [← hfg]
+        exact f.eval_codomain hxf
+      have hfxg' : f.eval x hxf ∈ g'.domain := by
+        rw [← hf'g']
+        rw [← hcodomff']
+        exact f.eval_codomain hxf
+      have hfxfx' : f.eval x hxf = f'.eval x hxf' := hff' hxf hxf'
+      have hgfxg'fx :
+        g.eval (f.eval x hxf) hfxg = g'.eval (f.eval x hxf) hfxg' :=
+        hgg' hfxg hfxg'
+      rw [hgfxg'fx]
+      have hf'xg' : f'.eval x hxf' ∈ g'.domain := by
+        rw [← hf'g']
+        exact f'.eval_codomain hxf'
+      exact g'.substitute hfxg' hf'xg' hfxfx'
 
 -- Exercise 3.3.2
 example (f : MyFun α β) (g : MyFun β γ)
   (hfg : f.codomain = g.domain) :
   f.isInjective → g.isInjective → (f.comp g hfg).isInjective := by
-  sorry
+  intro hf hg
+  dsimp only [MyFun.isInjective] at hf
+  dsimp only [MyFun.isInjective] at hg
+  dsimp only [MyFun.isInjective]
+  intro x x' hxgfdom hx'gfdom hxx'
+  dsimp only [MyFun.comp] at hxgfdom
+  dsimp only [MyFun.from_fun] at hxgfdom
+  dsimp only [MyFun.comp] at hx'gfdom
+  dsimp only [MyFun.from_fun] at hx'gfdom
+  have hfxgdom : f.eval x hxgfdom ∈ g.domain := by
+    rw [← hfg]
+    exact f.eval_codomain hxgfdom
+  rw [MyFun.comp.eval hfg hxgfdom hfxgdom]
+  have hfx'gdom : f.eval x' hx'gfdom ∈ g.domain := by
+    rw [← hfg]
+    exact f.eval_codomain hx'gfdom
+  rw [MyFun.comp.eval hfg hx'gfdom hfx'gdom]
+  exact hg hfxgdom hfx'gdom (hf hxgfdom hx'gfdom hxx')
 
 example (f : MyFun α β) (g : MyFun β γ)
   (hfg : f.codomain = g.domain) :
   f.isSurjective → g.isSurjective → (f.comp g hfg).isSurjective := by
-  sorry
+  intro hf hg
+  dsimp only [MyFun.isSurjective] at hf
+  dsimp only [MyFun.isSurjective] at hg
+  dsimp only [MyFun.isSurjective]
+  intro z hz
+  dsimp only [MyFun.comp] at hz
+  dsimp only [MyFun.from_fun] at hz
+  rcases hg z hz with ⟨y, hy, hgyz⟩
+  have hyfcodom : y ∈ f.codomain := by
+    rw [hfg]
+    exact hy
+  rcases hf y hyfcodom with ⟨x, hx, hfx⟩
+  use x, hx
+  have hfxgdom : f.eval x hx ∈ g.domain := by
+    rw [← hfg]
+    exact f.eval_codomain hx
+  rw [MyFun.comp.eval hfg hx hfxgdom]
+  rw [← hgyz]
+  exact g.substitute hfxgdom hy hfx
 
 -- Exercise 3.3.3
 -- TODO: When is the empty function into a given set X injective? surjective? bijective?
@@ -710,64 +820,326 @@ example (f : MyFun α β) (g : MyFun β γ)
 example (f f' : MyFun α β) (g : MyFun β γ)
   (hfg : f.codomain = g.domain) (hf'g : f'.codomain = g.domain) :
   (f.comp g hfg ≃ f'.comp g hf'g) → g.isInjective → f ≃ f' := by
-  sorry
+  intro hgfgf' hg
+  dsimp only [MyFun.eq] at hgfgf'
+  rcases hgfgf' with ⟨hgfgf'dom, hgfgf'codom, hgfgf'⟩
+  dsimp only [MyFun.comp] at hgfgf'dom
+  dsimp only [MyFun.from_fun] at hgfgf'dom
+  dsimp only [MyFun.eq]
+  constructor
+  · exact hgfgf'dom
+  · constructor
+    · rw [hfg]
+      rw [hf'g]
+    · intro x hxf hxf'
+      have hxgfdom : x ∈ (f.comp g hfg).domain := by
+        dsimp only [MyFun.comp]
+        dsimp only [MyFun.from_fun]
+        exact hxf
+      have hxgf'dom : x ∈ (f'.comp g hf'g).domain := by
+        dsimp only [MyFun.comp]
+        dsimp only [MyFun.from_fun]
+        exact hxf'
+      have hgfxgf'x :
+        (f.comp g hfg).eval x hxgfdom =
+          (f'.comp g hf'g).eval x hxgf'dom :=
+        hgfgf' hxgfdom hxgf'dom
+      have hfxgdom : f.eval x hxf ∈ g.domain := by
+        rw [← hfg]
+        exact f.eval_codomain hxf
+      rw [MyFun.comp.eval hfg hxf hfxgdom] at hgfxgf'x
+      have hfx'gdom : f'.eval x hxf' ∈ g.domain := by
+        rw [← hf'g]
+        exact f'.eval_codomain hxf'
+      rw [MyFun.comp.eval hf'g hxf' hfx'gdom] at hgfxgf'x
+      rw [MyFun.isInjective_iff] at hg
+      dsimp only [MyFun.isInjective'] at hg
+      exact hg hfxgdom hfx'gdom hgfxgf'x
 
 -- TODO: Is the same statement true if g is not injective?
 
 example (f : MyFun α β) (g g' : MyFun β γ)
   (hfg : f.codomain = g.domain) (hfg' : f.codomain = g'.domain) :
   (f.comp g hfg ≃ f.comp g' hfg') → f.isSurjective → g ≃ g' := by
-  sorry
+  intro hgfg'f hf
+  dsimp only [MyFun.eq] at hgfg'f
+  rcases hgfg'f with ⟨hgfg'fdom, hgfg'fcodom, hgfg'f⟩
+  dsimp only [MyFun.comp] at hgfg'fcodom
+  dsimp only [MyFun.from_fun] at hgfg'fcodom
+  dsimp only [MyFun.eq]
+  constructor
+  · rw [← hfg]
+    exact hfg'
+  · constructor
+    · exact hgfg'fcodom
+    · intro y hygdom hyg'dom
+      dsimp only [MyFun.isSurjective] at hf
+      have hyfcodom : y ∈ f.codomain := by
+        rw [hfg]
+        exact hygdom
+      rcases hf y hyfcodom with ⟨x, hxf, hfy⟩
+      have hfxgdom : f.eval x hxf ∈ g.domain := by
+        rw [← hfg]
+        exact f.eval_codomain hxf
+      have hfxg'dom : f.eval x hxf ∈ g'.domain := by
+        rw [← hfg']
+        exact f.eval_codomain hxf
+      have hgfxg'fx :
+        (f.comp g hfg).eval x hxf =
+          (f.comp g' hfg').eval x hxf :=
+        hgfg'f hxf hxf
+      rw [MyFun.comp.eval hfg hxf hfxgdom] at hgfxg'fx
+      rw [MyFun.comp.eval hfg' hxf hfxg'dom] at hgfxg'fx
+      have hgfxgy :
+        g.eval (f.eval x hxf) hfxgdom = g.eval y hygdom :=
+        g.substitute hfxgdom hygdom hfy
+      have hg'fxg'y :
+        g'.eval (f.eval x hxf) hfxg'dom = g'.eval y hyg'dom :=
+        g'.substitute hfxg'dom hyg'dom hfy
+      rw [← hgfxgy]
+      rw [← hg'fxg'y]
+      exact hgfxg'fx
 
 -- TODO: Is the same statement true if f is not surjective?
 
 -- Exercise 3.3.5
 example (f : MyFun α β) (g : MyFun β γ) (hfg : f.codomain = g.domain) :
   (f.comp g hfg).isInjective → f.isInjective := by
-  sorry
+  intro hgf
+  dsimp only [MyFun.isInjective] at hgf
+  dsimp only [MyFun.isInjective]
+  intro x x' hxfdom hx'fdom hxx'
+  have hxgfdom : x ∈ (f.comp g hfg).domain := by
+    dsimp only [MyFun.comp]
+    dsimp only [MyFun.from_fun]
+    exact hxfdom
+  have hx'gfdom : x' ∈ (f.comp g hfg).domain := by
+    dsimp only [MyFun.comp]
+    dsimp only [MyFun.from_fun]
+    exact hx'fdom
+  have hgfxngfx' := hgf hxgfdom hx'gfdom hxx'
+  have hfxgdom : f.eval x hxfdom ∈ g.domain := by
+    rw [← hfg]
+    exact f.eval_codomain hxfdom
+  have hfx'gdom : f.eval x' hx'fdom ∈ g.domain := by
+    rw [← hfg]
+    exact f.eval_codomain hx'fdom
+  rw [MyFun.comp.eval hfg hxfdom hfxgdom] at hgfxngfx'
+  rw [MyFun.comp.eval hfg hx'fdom hfx'gdom] at hgfxngfx'
+  intro hfxfx'
+  have hgfxgfx' :
+    g.eval (f.eval x hxfdom) hfxgdom
+      = g.eval (f.eval x' hx'fdom) hfx'gdom :=
+    g.substitute hfxgdom hfx'gdom hfxfx'
+  exact hgfxngfx' hgfxgfx'
 
 -- TODO: Is it true that g must also be injective?
 
 example (f : MyFun α β) (g : MyFun β γ) (hfg : f.codomain = g.domain) :
   (f.comp g hfg).isSurjective → g.isSurjective := by
-  sorry
+  intro hgf
+  dsimp only [MyFun.isSurjective] at hgf
+  dsimp only [MyFun.isSurjective]
+  intro z hz
+  have hzgfcodom : z ∈ (f.comp g hfg).codomain := by
+    dsimp only [MyFun.comp]
+    dsimp only [MyFun.from_fun]
+    exact hz
+  rcases hgf z hzgfcodom with ⟨x, hxgfdom, hgfxz⟩
+  have hxfdom : x ∈ f.domain := by
+    dsimp only [MyFun.comp] at hxgfdom
+    dsimp only [MyFun.from_fun] at hxgfdom
+    exact hxgfdom
+  have hfxgdom : f.eval x hxfdom ∈ g.domain := by
+    rw [← hfg]
+    exact f.eval_codomain hxfdom
+  use (f.eval x hxfdom), hfxgdom
+  rw [MyFun.comp.eval hfg hxfdom hfxgdom] at hgfxz
+  exact hgfxz
 
 -- TODO: Is it true that f must also be surjective?
 
 -- Exercise 3.3.6
 namespace Exercise_3_3_6
 
-lemma aux₁ {f : MyFun α β} (hf : f.isBijective)
-  {fi : MyFun β α} (hfi : fi = MyFun.inv f hf) :
-  f.codomain = fi.domain := by
-  sorry
+lemma aux₁ {f : MyFun α β} (hf : f.isBijective) :
+  f.codomain = (f.inv hf).domain := by
+  dsimp only [MyFun.inv]
+  dsimp only [MyFun.from_fun]
 
-example (f : MyFun α β) (hf : f.isBijective)
-  {fi : MyFun β α} (hfi : fi = MyFun.inv f hf) :
-  ∀ (x : α) (hx : x ∈ f.domain),
-    (f.comp fi (aux₁ hf hfi)).eval x hx = x := by
-  sorry
+lemma finv_f {f : MyFun α β} (hf : f.isBijective) :
+  ∀ {x : α} (hx : x ∈ f.domain),
+    (f.comp (f.inv hf) (aux₁ hf)).eval x hx = x := by
+  intro x hxf
+  have hffi : f.codomain = (f.inv hf).domain := aux₁ hf
+  have hfxfidom : f.eval x hxf ∈ (f.inv hf).domain := by
+    rw [← hffi]
+    exact f.eval_codomain hxf
+  rw [MyFun.comp.eval hffi hxf hfxfidom]
+  dsimp only [MyFun.inv]
+  rw [MyFun.from_fun.eval]
+  rcases (MyFun.exists_unique_of_bijective hf hfxfidom).choose_spec
+    with ⟨hx, h, h'⟩
+  exact h' hxf rfl
 
-lemma aux₂ {f : MyFun α β} (hf : f.isBijective)
-  {fi : MyFun β α} (hfi : fi = MyFun.inv f hf) :
-  fi.codomain = f.domain := by
-  sorry
+lemma aux₂ {f : MyFun α β} (hf : f.isBijective) :
+  (f.inv hf).codomain = f.domain := by
+  dsimp only [MyFun.inv]
+  dsimp only [MyFun.from_fun]
 
-example (f : MyFun α β) (hf : f.isBijective)
-  {fi : MyFun β α} (hfi : fi = MyFun.inv f hf) :
-  ∀ (y : β) (hy : y ∈ fi.domain),
-    (fi.comp f (aux₂ hf hfi)).eval y hy = y := by
-  sorry
+lemma f_finv {f : MyFun α β} (hf : f.isBijective) :
+  ∀ {y : β} (hy : y ∈ (f.inv hf).domain),
+    ((f.inv hf).comp f (aux₂ hf)).eval y hy = y := by
+  intro y hyfidom
+  have hffi : (f.inv hf).codomain = f.domain := aux₂ hf
+  have hfiyfdom : (f.inv hf).eval y hyfidom ∈ f.domain := by
+    rw [← hffi]
+    exact (f.inv hf).eval_codomain hyfidom
+  rw [MyFun.comp.eval hffi hyfidom hfiyfdom]
+  dsimp only [MyFun.inv] at hyfidom
+  dsimp only [MyFun.from_fun] at hyfidom
+  rcases (MyFun.exists_unique_of_bijective hf hyfidom).choose_spec
+    with ⟨hx, h, h'⟩
+  have hPfiyy : f.prop ((f.inv hf).eval y hyfidom) y := by
+    dsimp only [MyFun.inv]
+    rw [MyFun.from_fun.eval]
+    have := (MyFun.def f hx hyfidom).mp
+    exact this h.symm
+  have := (MyFun.def f hfiyfdom hyfidom).mpr hPfiyy
+  exact this.symm
 
-lemma aux {f : MyFun α β} (hf : f.isBijective)
-  {fi : MyFun β α} (hfi : fi = MyFun.inv f hf) :
-  fi.isBijective := by
-  sorry
+lemma finv_bij {f : MyFun α β} (hf : f.isBijective) :
+  (f.inv hf).isBijective := by
+  have hf : f.isBijective := hf
+  dsimp only [MyFun.isBijective] at hf
+  rcases hf with ⟨hinj, hsurj⟩
+  dsimp only [MyFun.isBijective]
+  constructor
+  · dsimp only [MyFun.isInjective]
+    intro y y' hy hy' hyy'
+    intro hfiyfiy'
+    dsimp only [MyFun.isSurjective] at hsurj
+    have hyfcodom : y ∈ f.codomain := by
+      dsimp only [MyFun.inv] at hy
+      dsimp only [MyFun.from_fun] at hy
+      exact hy
+    rcases hsurj y hyfcodom with ⟨x, hxfdom, hfxy⟩
+    have hy'fcodom : y' ∈ f.codomain := by
+      dsimp only [MyFun.inv] at hy'
+      dsimp only [MyFun.from_fun] at hy'
+      exact hy'
+    rcases hsurj y' hy'fcodom with ⟨x', hx'fdom, hfx'y'⟩
+    have hfxfidom : (f.eval x hxfdom) ∈ (f.inv hf).domain := by
+      dsimp only [MyFun.inv]
+      dsimp only [MyFun.from_fun]
+      exact f.eval_codomain hxfdom
+    have hfiyfifx :
+      (f.inv hf).eval y hy =
+        (f.inv hf).eval (f.eval x hxfdom) hfxfidom :=
+      MyFun.substitute (f.inv hf) hy hfxfidom hfxy.symm
+    rw [hfiyfifx] at hfiyfiy'
+    have hfx'fidom : (f.eval x' hx'fdom) ∈ (f.inv hf).domain := by
+      dsimp only [MyFun.inv]
+      dsimp only [MyFun.from_fun]
+      exact f.eval_codomain hx'fdom
+    have hfiy'fifx' :
+      (f.inv hf).eval y' hy' =
+        (f.inv hf).eval (f.eval x' hx'fdom) hfx'fidom :=
+      MyFun.substitute (f.inv hf) hy' hfx'fidom hfx'y'.symm
+    rw [hfiy'fifx'] at hfiyfiy'
+    have hxfifdom : x ∈ (f.comp (f.inv hf) (aux₁ hf)).domain := by
+      dsimp only [MyFun.comp]
+      dsimp only [MyFun.from_fun]
+      exact hxfdom
+    rw [← MyFun.comp.eval (aux₁ hf) hxfdom hfxfidom hxfifdom] at hfiyfiy'
+    have hx'fifdom : x' ∈ (f.comp (f.inv hf) (aux₁ hf)).domain := by
+      dsimp only [MyFun.comp]
+      dsimp only [MyFun.from_fun]
+      exact hx'fdom
+    rw [← MyFun.comp.eval (aux₁ hf) hx'fdom hfx'fidom hx'fifdom] at hfiyfiy'
+    rw [finv_f hf hxfdom] at hfiyfiy'
+    rw [finv_f hf hx'fdom] at hfiyfiy'
+    have hfxfx' : f.eval x hxfdom = f.eval x' hx'fdom :=
+      MyFun.substitute f hxfdom hx'fdom hfiyfiy'
+    rw [hfxy] at hfxfx'
+    rw [hfx'y'] at hfxfx'
+    exact hyy' hfxfx'
+  · dsimp only [MyFun.isSurjective]
+    intro x hxficodom
+    have hxfdom : x ∈ f.domain := by
+      dsimp only [MyFun.inv]
+      exact hxficodom
+    use (f.eval x hxficodom)
+    have hfxfidom : f.eval x hxfdom ∈ (f.inv hf).domain := by
+      dsimp only [MyFun.inv]
+      dsimp only [MyFun.from_fun]
+      exact f.eval_codomain hxfdom
+    use hfxfidom
+    have hxfifdom : x ∈ (f.comp (f.inv hf) (aux₁ hf)).domain := by
+      dsimp only [MyFun.comp]
+      dsimp only [MyFun.from_fun]
+      exact hxfdom
+    rw [← MyFun.comp.eval (aux₁ hf) hxfdom hfxfidom hxfifdom]
+    rw [finv_f hf hxfdom]
 
-example (f : MyFun α β) (hf : f.isBijective)
-  {fi : MyFun β α} (hfi : fi = MyFun.inv f hf) :
-  fi.inv (aux hf hfi) ≃ f := by
-  sorry
+example (f : MyFun α β) (hf : f.isBijective) :
+  (f.inv hf).inv (finv_bij hf) ≃ f := by
+  have hfi : (f.inv hf).isBijective := finv_bij hf
+  dsimp only [MyFun.eq]
+  constructor
+  · dsimp only [MyFun.inv]
+    dsimp only [MyFun.from_fun]
+  · constructor
+    · dsimp only [MyFun.inv]
+      dsimp only [MyFun.from_fun]
+    · intro x hxfiidom hxfdom
+      have hfiicodomfidom :
+        ((f.inv hf).inv hfi).codomain = (f.inv hf).domain := by
+        dsimp only [MyFun.inv]
+        dsimp only [MyFun.from_fun]
+      have hxfifiidom :
+        x ∈ (((f.inv hf).inv hfi).comp (f.inv hf) hfiicodomfidom).domain := by
+        dsimp only [MyFun.comp]
+        dsimp only [MyFun.from_fun]
+        exact hxfiidom
+      have hxfifdom :
+        x ∈ (f.comp (f.inv hf) (aux₁ hf)).domain := by
+        dsimp only [MyFun.comp]
+        dsimp only [MyFun.from_fun]
+        exact hxfdom
+      have hfifiixfifx:
+        (((f.inv hf).inv hfi).comp (f.inv hf) hfiicodomfidom).eval x hxfifiidom =
+          (f.comp (f.inv hf) (aux₁ hf)).eval x hxfifdom := by
+        have hxfiidom : x ∈ ((f.inv hf).inv hfi).domain := by
+          dsimp only [MyFun.inv]
+          dsimp only [MyFun.from_fun]
+          exact hxfiidom
+        rw [f_finv hfi hxfiidom]
+        rw [finv_f hf hxfiidom]
+      have hfiixfidom :
+        ((f.inv hf).inv hfi).eval x hxfifiidom ∈ (f.inv hf).domain := by
+        have hfiixfiicodom:
+          ((f.inv hf).inv hfi).eval x hxfifiidom ∈ ((f.inv hf).inv hfi).codomain :=
+          ((f.inv hf).inv hfi).eval_codomain hxfifiidom
+        have hfiicodomfidom :
+          ((f.inv hf).inv hfi).codomain = (f.inv hf).domain := by
+          dsimp only [MyFun.inv]
+          dsimp only [MyFun.from_fun]
+        rw [← hfiicodomfidom]
+        exact hfiixfiicodom
+      have hfxfidom :
+        f.eval x hxfifdom ∈ (f.inv hf).domain := by
+        dsimp only [MyFun.inv]
+        dsimp only [MyFun.from_fun]
+        exact f.eval_codomain hxfdom
+      rw [MyFun.comp.eval hfiicodomfidom hxfifiidom hfiixfidom] at hfifiixfifx
+      rw [MyFun.comp.eval (aux₁ hf) hxfifdom hfxfidom] at hfifiixfifx
+      have hfi := hfi
+      dsimp only [MyFun.isBijective] at hfi
+      rcases hfi with ⟨hfi_inj, hfi_surj⟩
+      rw [(f.inv hf).isInjective_iff] at hfi_inj
+      dsimp only [MyFun.isInjective'] at hfi_inj
+      exact hfi_inj hfiixfidom hfxfidom hfifiixfifx
 
 end Exercise_3_3_6
 
@@ -777,18 +1149,181 @@ namespace Exercise_3_3_7
 lemma aux₁ {f : MyFun α β} {g : MyFun β γ} (hfg : f.codomain = g.domain)
   (hf : f.isBijective) (hg : g.isBijective) :
   (f.comp g hfg).isBijective := by
-  sorry
+  dsimp only [MyFun.isBijective]
+  constructor
+  · dsimp only [MyFun.isInjective]
+    intro x x' hxgfdom hx'gfdom hxnx'
+    intro hgfxgfx'
+    have hxfdom : x ∈ f.domain := by
+      dsimp only [MyFun.comp] at hxgfdom
+      dsimp only [MyFun.from_fun] at hxgfdom
+      exact hxgfdom
+    have hfxgdom : f.eval x hxfdom ∈ g.domain := by
+      rw [← hfg]
+      exact f.eval_codomain hxfdom
+    rw [MyFun.comp.eval hfg hxfdom hfxgdom] at hgfxgfx'
+    have hx'fdom : x' ∈ f.domain := by
+      dsimp only [MyFun.comp] at hx'gfdom
+      dsimp only [MyFun.from_fun] at hx'gfdom
+      exact hx'gfdom
+    have hfx'gdom : f.eval x' hx'fdom ∈ g.domain := by
+      rw [← hfg]
+      exact f.eval_codomain hx'fdom
+    rw [MyFun.comp.eval hfg hx'fdom hfx'gdom] at hgfxgfx'
+    dsimp only [MyFun.isBijective] at hg
+    rcases hg with ⟨hg_inj, hg_surj⟩
+    rw [g.isInjective_iff] at hg_inj
+    dsimp only [MyFun.isInjective'] at hg_inj
+    have hfxfx' : f.eval x hxfdom = f.eval x' hx'fdom :=
+      hg_inj hfxgdom hfx'gdom hgfxgfx'
+    dsimp only [MyFun.isBijective] at hf
+    rcases hf with ⟨hf_inj, hf_surj⟩
+    rw [f.isInjective_iff] at hf_inj
+    dsimp only [MyFun.isInjective'] at hf_inj
+    have hxx' := hf_inj hxfdom hx'fdom hfxfx'
+    exact hxnx' hxx'
+  · dsimp only [MyFun.isSurjective]
+    intro z hzgfcodom
+    dsimp only [MyFun.isBijective] at hg
+    rcases hg with ⟨hg_inj, hg_surj⟩
+    dsimp only [MyFun.isSurjective] at hg_surj
+    rcases hg_surj z hzgfcodom with ⟨y, hygdom, hgyz⟩
+    dsimp only [MyFun.isBijective] at hf
+    rcases hf with ⟨hf_inj, hf_surj⟩
+    dsimp only [MyFun.isSurjective] at hf_surj
+    have hyfcodom : y ∈ f.codomain := by
+      rw [hfg]
+      exact hygdom
+    rcases hf_surj y hyfcodom with ⟨x, hxfdom, hfyx⟩
+    use x
+    have hxgfdom : x ∈ (f.comp g hfg).domain := by
+      dsimp only [MyFun.comp]
+      dsimp only [MyFun.from_fun]
+      exact hxfdom
+    use hxgfdom
+    have hfxgdom : f.eval x hxfdom ∈ g.domain := by
+      rw [← hfg]
+      exact f.eval_codomain hxfdom
+    rw [MyFun.comp.eval hfg hxfdom hfxgdom]
+    rw [← hgyz]
+    exact g.substitute hfxgdom hygdom hfyx
 
 lemma aux₂ {f : MyFun α β} {g : MyFun β γ} (hfg : f.codomain = g.domain)
   (hf : f.isBijective) (hg : g.isBijective) :
   (g.inv hg).codomain = (f.inv hf).domain := by
-  sorry
+  dsimp only [MyFun.inv]
+  dsimp only [MyFun.from_fun]
+  exact hfg.symm
 
 example (f : MyFun α β) (g : MyFun β γ) (hfg : f.codomain = g.domain)
   (hf : f.isBijective) (hg : g.isBijective) :
   (f.comp g hfg).inv (aux₁ hfg hf hg) ≃
     (g.inv hg).comp (f.inv hf) (aux₂ hfg hf hg) := by
-  sorry
+  dsimp only [MyFun.eq]
+  constructor
+  · dsimp only [MyFun.inv]
+    dsimp only [MyFun.comp]
+    dsimp only [MyFun.from_fun]
+  · constructor
+    · dsimp only [MyFun.inv]
+      dsimp only [MyFun.comp]
+      dsimp only [MyFun.from_fun]
+    · intro z hzgfidom hzfigidom
+      have hzgidom : z ∈ (g.inv hg).domain := by
+        dsimp only [MyFun.inv]
+        dsimp only [MyFun.from_fun]
+        dsimp only [MyFun.inv] at hzgfidom
+        dsimp only [MyFun.from_fun] at hzgfidom
+        dsimp only [MyFun.comp] at hzgfidom
+        dsimp only [MyFun.from_fun] at hzgfidom
+        exact hzgfidom
+      have hgizfidom : (g.inv hg).eval z hzgidom ∈ (f.inv hf).domain := by
+        have : (f.inv hf).domain = (g.inv hg).codomain := by
+          dsimp only [MyFun.inv]
+          dsimp only [MyFun.from_fun]
+          exact hfg
+        rw [this]
+        exact (g.inv hg).eval_codomain hzgidom
+      rw [MyFun.comp.eval (aux₂ hfg hf hg) hzgfidom hgizfidom]
+      have hg : g.isBijective := hg
+      dsimp only [MyFun.isBijective] at hg
+      rcases hg with ⟨hg_inj, hg_surj⟩
+      dsimp only [MyFun.isSurjective] at hg_surj
+      have hzgcodom : z ∈ g.codomain := by
+        dsimp only [MyFun.inv] at hzgfidom
+        dsimp only [MyFun.from_fun] at hzgfidom
+        dsimp only [MyFun.comp] at hzgfidom
+        dsimp only [MyFun.from_fun] at hzgfidom
+        exact hzgfidom
+      rcases MyFun.exists_unique_of_bijective hg hzgfidom with ⟨y, hygdom, hgyz, hgyz!⟩
+      have hgizy : (g.inv hg).eval z hzgfidom = y := by
+        have hgygidom : g.eval y hygdom ∈ (g.inv hg).domain := by
+          have : (g.inv hg).domain = g.codomain := by
+            dsimp only [MyFun.inv]
+            dsimp only [MyFun.from_fun]
+          rw [this]
+          exact g.eval_codomain hygdom
+        have :
+          (g.inv hg).eval z hzgfidom =
+            (g.inv hg).eval (g.eval y hygdom) hgygidom :=
+          MyFun.substitute (g.inv hg) hzgfidom hgygidom hgyz.symm
+        rw [this]
+        rw [← MyFun.comp.eval]
+        exact Exercise_3_3_6.finv_f hg hygdom
+      have hyfidom : y ∈ (f.inv hf).domain := by
+        dsimp only [MyFun.inv]
+        dsimp only [MyFun.from_fun]
+        rw [hfg]
+        exact hygdom
+      rw [MyFun.substitute (f.inv hf) hgizfidom hyfidom hgizy]
+      rcases MyFun.exists_unique_of_bijective hf hyfidom with ⟨x, hxfdom, hfxz, hfxz!⟩
+      have hfiyx : (f.inv hf).eval y hyfidom = x := by
+        have hfxgidom : f.eval x hxfdom ∈ (f.inv hf).domain := by
+          have : (f.inv hf).domain = f.codomain := by
+            dsimp only [MyFun.inv]
+            dsimp only [MyFun.from_fun]
+          rw [this]
+          exact f.eval_codomain hxfdom
+        have :
+          (f.inv hf).eval y hyfidom =
+            (f.inv hf).eval (f.eval x hxfdom) hfxgidom :=
+          MyFun.substitute (f.inv hf) hyfidom hfxgidom hfxz.symm
+        rw [this]
+        rw [← MyFun.comp.eval]
+        exact Exercise_3_3_6.finv_f hf hxfdom
+      rw [hfiyx]
+      have hgf : (f.comp g hfg).isBijective := aux₁ hfg hf hg
+      rcases MyFun.exists_unique_of_bijective hgf hzgfidom with ⟨x', hx'gfdom, hgfx'z, hgfx'z!⟩
+
+      have hgfx'gfidom : (f.comp g hfg).eval x' hx'gfdom ∈ ((f.comp g hfg).inv hgf).domain := by
+        have : ((f.comp g hfg).inv hgf).domain = (f.comp g hfg).codomain := by
+          dsimp only [MyFun.inv]
+          dsimp only [MyFun.comp]
+          dsimp only [MyFun.from_fun]
+        rw [this]
+        exact (f.comp g hfg).eval_codomain hx'gfdom
+      have :
+        ((f.comp g hfg).inv hgf).eval z hzgfidom =
+          ((f.comp g hfg).inv hgf).eval ((f.comp g hfg).eval x' hx'gfdom) hgfx'gfidom :=
+        ((f.comp g hfg).inv hgf).substitute hzgfidom hgfx'gfidom hgfx'z.symm
+      rw [this]
+      have : x' ∈ (f.comp g hfg).domain := hx'gfdom
+      rw [← MyFun.comp.eval]
+      rw [Exercise_3_3_6.finv_f hgf hx'gfdom]
+      have hxgfdom : x ∈ (f.comp g hfg).domain := by
+        dsimp only [MyFun.comp]
+        dsimp only [MyFun.from_fun]
+        exact hxfdom
+      have hgfxz : (f.comp g hfg).eval x hxgfdom = z := by
+        have hfxgdom : f.eval x hxfdom ∈ g.domain := by
+          rw [← hfg]
+          exact f.eval_codomain hxfdom
+        rw [MyFun.comp.eval hfg hxfdom hfxgdom]
+        have : g.eval (f.eval x hxfdom) hfxgdom = g.eval y hygdom :=
+          g.substitute hfxgdom hygdom hfxz
+        rw [this]
+        exact hgyz
+      exact hgfx'z! hxgfdom hgfxz
 
 end Exercise_3_3_7
 
